Serious rewrite w/ debruijn constructors, etc

coq/CoreDefs.v
@@ -5,29 +5,419 @@ Unset Strict Implicit.
 Unset Printing Implicit Defensive.
 Set Bullet Behavior "Strict Subproofs".
 
-(* TODO: change from loads to imports*)
 From excomp Require Import Exp.
+
+Tactic Notation "intro_to" constr(ty) :=
+  repeat match goal with
+         | |- ty -> _ => idtac
+         | |- ty _ -> _ => idtac
+         | |- ty _ _-> _ => idtac
+         | |- ty _ _ _ -> _ => idtac
+         | |- _ -> _ => intro
+         end.
+
+(* grouped right with the fixpoint so that eq_exp goes through*)
+Definition all2 := 
+fun (S T : Type) (r : S -> T -> bool) =>
+fix all2 (s : seq S) (t : seq T) {struct s} : bool :=
+  match s, t with
+  | [::], [::] => true
+  | x :: s0, y::t0 => r x y && all2 s0 t0
+  | _,_ => false
+  end.
+
+(* TODO: I have to inline all2 to get this accepted *)
+Fixpoint eq_exp e1 e2 {struct e1} : bool :=
+  match e1, e2 with
+  | var x, var y => x == y
+  | con n1 l1, con n2 l2 =>
+    (n1 == n2) && (all2 eq_exp l1 l2)
+  | _,_ => false
+  end.
+
+Lemma all2P {T} eqb (l1 l2 : seq T)
+  : (forall e1 e2, reflect (e1 = e2) (eqb e1 e2)) ->
+    reflect (l1 = l2) (all2 eqb l1 l2).
+Proof.
+  move => eqbP.
+  elim: l1 l2.
+  - case; simpl; [by constructor|].
+    intros.
+    constructor; eauto.
+    move => H; inversion H.
+  - move => a l IH.
+    case; simpl.
+    constructor; move => H; inversion H.
+    intros.
+    move: (eqbP a a0).
+    case (eqb a a0); simpl.
+    move: (IH l0); case:(all2 eqb l l0); simpl.
+    + constructor.
+      inversion IH0; inversion eqbP0; by subst.
+    + constructor.
+      move => lfl.
+      inversion lfl.
+      inversion IH0; eauto.
+    + constructor; move => lfl.
+      inversion lfl; inversion eqbP0; auto.
+Qed.
+
+Lemma exp2_ind (P : exp -> exp -> Set)
+  : (forall n m, P (var n) (var m)) ->
+    (forall n c l, P (var n) (con c l)) ->
+    (forall n c l, P (con c l) (var n)) ->
+    (forall c1 c2, P (con c1 [::]) (con c2 [::])) ->
+    (forall c1 c2 a l, P (con c1 [::]) (con c2 (a::l))) ->
+    (forall c1 c2 a l, P (con c1 (a::l)) (con c2 [::])) ->
+    (forall c1 c2 a1 a2 l1 l2,
+        P a1 a2 ->
+        P (con c1 l1) (con c2 l2) ->
+        P (con c1 (a1::l1)) (con c2 (a2::l2))) ->
+    forall e1 e2, P e1 e2.
+Proof.
+  intro_to exp.
+  elim.
+  - intro_to exp; case; auto.
+  - intro_to exp.
+    case; auto.
+    move => n0.
+    elim: l X.
+    + move => _; case; auto.
+    + move => a l IH.
+      simpl; case => pa fld.
+      case; auto.
+Qed.      
+
+Tactic Notation "case_on_eqb" ident(a) ident(b) :=
+  let neq := fresh "neq" in
+  case neq: (a == b); constructor;
+  [f_equal; apply /eqP
+  | case => /eqP; rewrite neq].
+  
+
+Lemma eq_exp_refl : forall e, eq_exp e e.
+Proof.
+  elim; simpl; auto.
+  move => n.
+  suff: n == n.
+  move ->; simpl.
+  elim; simpl; auto.
+  intro_to and.
+  case => eqaa fld.
+  apply /andP.
+  split; auto.
+  elim: n; simpl; auto.
+Qed.
+
+Lemma all2_eq_exp_refl : forall l, all2 eq_exp l l.
+  pose eqer := eq_exp_refl.
+  elim; simpl; auto.
+  intros; apply /andP; split; auto.
+Qed.
+
+Lemma eq_expP : forall e1 e2, reflect (e1 = e2) (eq_exp e1 e2).
+Proof.
+  elim.
+  - intro_to exp; case; simpl.
+    + move => n0.
+        by case_on_eqb n n0.
+    + constructor; by case.
+  - intro_to exp; case; simpl.
+    + constructor; by case.
+    + intros.
+      case neq: (n == n0); simpl.
+      * case alleq: (all2 eq_exp l l0).
+        --constructor.
+          f_equal.
+            by apply /eqP; rewrite neq.
+            elim: l X l0 alleq.
+          ++ simpl; move => _; case; by auto.
+          ++ simpl; move => a l IH.
+             case => refla fld.
+             case; try by auto.
+             move => a0 l0.
+             case /andP.
+             move /refla => -> all2l.
+             f_equal.
+             eauto.
+        -- constructor.
+           case => _.
+           elim: l X l0 alleq.
+           ++ simpl; move => _; case; by auto.
+          ++ simpl; move => a l IH.
+             case => refla fld.
+             case; try by auto.
+             move => a0 l0.
+             move /andP => oneof.
+             case => aeq leq.
+             apply oneof.
+             split.
+             rewrite aeq.
+             apply: eq_exp_refl.
+             rewrite leq.
+             apply: all2_eq_exp_refl.
+      * constructor.
+        case; move /eqP; by rewrite neq.
+Qed.
+
+Definition exp_eqMixin := Equality.Mixin eq_expP.
+
+Canonical exp_eqType := @Equality.Pack exp exp_eqMixin.
+
+(* TODO: necessary for computational defn
+Lemma eq_expP e1 e2 : reflect (e1 = e2) (eq_exp e1 e2).
+Proof.
+  elim: e1 e2; intro_to exp; elim; intros; simpl; eauto.
+  - case neq : (n == n0); constructor.
+    + f_equal; by apply: eqP.
+    + case.
+      move /eqP.
+        by rewrite neq.
+  - constructor => //.
+  - constructor => //.
+  - case neq: (n == n0); simpl.
+    + elim: l l0.
+      * case; simpl; constructor; f_equal.
+        apply /eqP; eauto.
+        case => _.
+        case => //.
+      * move => a l IH.
+        case.
+        -- constructor; by case.
+        -- intros.
+           case eqa: (eq_exp a a0); simpl.
+           give_up.
+           ++ constructor.
+              case => _.
+              
+    + constructor.
+      case.
+      move /eqP.
+        by rewrite neq.
+Qed.
+*)
+
+Definition eq_rule r1 r2 : bool :=
+  match r1, r2 with
+  | {| c1 |- sort }, {| c2 |- sort } => c1 == c2
+  | {| c1 |- t1 }, {| c2 |- t2 } => (c1 == c2) && (t1 == t2)
+  | {< c1 <# c2 |- t1 <# t2 },{< c1' <# c2' |- t1' <# t2' } =>
+    (c1 == c1') && (t1 == t1') && (c2 == c2') && (t2 == t2')
+  | {< c1 <# c2 |- e1 <# e2 .: t1 <# t2 },{< c1' <# c2' |- e1' <# e2' .: t1' <# t2' } =>
+    (c1 == c1') && (e1 == e1') && (t1 == t1') && (c2 == c2')  && (e2 == e2') && (t2 == t2')
+  | _,_ => false
+  end.
+
+Tactic Notation "inversion" :=
+  let H := fresh in
+  move => H; inversion H.
+
+Lemma eq_ruleP r1 r2 : reflect (r1 = r2) (eq_rule r1 r2).
+Proof.
+  case: r1 r2; intro_to rule; case; intros; simpl; eauto;
+  try match goal with
+  | |- reflect _ false => constructor; by inversion
+  | |- reflect _ (?A == ?B) =>
+    case eqcase: (A == B); constructor;
+      solve [ by f_equal; apply /eqP
+            | by case; move /eqP; rewrite eqcase]
+      end.
+  match goal with
+  | |- reflect _ (?E && _) => case and1: E; simpl
+  end.
+  match goal with
+  | |- reflect _ false => constructor; by inversion
+  | |- reflect _ (?A == ?B) =>
+    case eqcase: (A == B); constructor;
+      try solve [ by f_equal; apply /eqP
+            | by case; move /eqP; rewrite eqcase]
+  end.
+Admitted.
+
+Definition rule_eqMixin := Equality.Mixin eq_ruleP.
+
+Canonical rule_eqType := @Equality.Pack rule rule_eqMixin.
+
+
+(*TODO: move these to Exp*)
+Fixpoint constr_shift n e :=
+  match e with
+  | var x => var x
+  | con m l => con (n + m) (map (constr_shift n) l)
+  end.
+
+
+Notation "e %! n" := (constr_shift n e) (at level 7).
+
+Notation "e ::%! n" := (map (constr_shift n) e) (at level 7).
+
+Lemma constr_shift0 e : e%!0 = e.
+Proof.
+  elim: e => //.
+  intros; simpl.
+  f_equal.
+  elim: l H => //.
+  simpl; intros.
+  case: H0 => H01 H02; f_equal; auto.
+Qed.
+
+Lemma map_constr_shift0 s : s::%!0 = s.
+  elim: s => //.
+  intros; simpl; f_equal; move: constr_shift0; auto.
+Qed.
+  
+Lemma constr_shift_shift e n m : e%!n %!m = e%!(n + m).
+Proof.
+  elim: e => //.
+  intros;
+    simpl;
+    f_equal.
+  - ring.
+  - elim: l H => //; simpl; intros.
+    rewrite -> H;
+      case: H0; intros.
+    f_equal; auto.
+    auto.
+Qed.
+
+Definition rule_constr_shift n r :=
+  match r with
+  | {| c |- sort } => {| map (constr_shift n) c |- sort}
+  | {| c |- t } => {| map (constr_shift n) c |- constr_shift n t}
+  | {< c1 <# c2 |- t1 <# t2 } =>
+    {< map (constr_shift n) c1 <# map (constr_shift n) c2
+     |- constr_shift n t1 <# constr_shift n t2 }
+  | {< c1 <# c2 |- e1 <# e2 .: t1 <# t2 } =>
+    {< map (constr_shift n) c1 <# map (constr_shift n) c2
+     |- constr_shift n e1 <# constr_shift n e2
+                     .: constr_shift n t1 <# constr_shift n t2}
+  end.
+
+Notation "r %%! n" := (rule_constr_shift n r) (at level 7).
+
+(*TODO: should be mutually recursive w/ last lemma *)
+Lemma map_constr_shift_shift l n m
+  : [seq e%!m | e <- [seq e'%!n | e' <- l]] = [seq e%!(n + m) | e <- l].
+Proof.
+  elim: l => //.
+  simpl.
+  move => a l ->.
+  f_equal; move: constr_shift_shift; auto.
+Qed.
+
+Lemma rule_constr_shift_shift r n m : r%%!n %%!m = r%%!(n+m).
+Proof.
+  case: r; simpl; intros; f_equal;
+    move: constr_shift_shift map_constr_shift_shift;
+  auto.
+Qed.
+
+Lemma constr_shift_subst_comm e s n : e[/s/]%!n = e%!n[/s::%!n/].
+Proof.
+  elim: e s n.
+  - elim ;intro_to subst; case => //.
+  - intros; simpl;
+      unfold exp_subst;
+      unfold exp_var_map;
+      fold exp_var_map;
+      fold exp_subst.
+    f_equal.
+    fold exp_subst.
+    elim: l H => //.
+    simpl; intro_to and.
+    case; intros.
+    f_equal; eauto.
+Qed.
+
+(* determines whether a given language contains the appropriate axiom.
+   Uses constructor shifts to get the right debruijn indices
+ *)
+Fixpoint shifted_rule_in n (r : rule) (l : lang) : bool :=
+  match l with
+  | [::] => false
+  | r' :: l' => ( r' %%! n == r) || (shifted_rule_in (n.+1) r l')
+  end.
+
+Lemma shifted_rule_in_cons n r l
+  : shifted_rule_in n.+1 r l -> forall r', shifted_rule_in n r (r'::l).
+Proof.
+  intros; by apply /orP; auto.
+Qed.
+
+Lemma unshift_rule_in_cons n r l
+  : shifted_rule_in n r l -> forall m, shifted_rule_in (n + m) r%%!m l.
+Proof.
+  elim: l n => //.
+  intro_to is_true.
+  case /orP => [ /eqP <- |].
+  - move => m; rewrite rule_constr_shift_shift.
+    simpl.
+    apply /orP; left; by apply /eqP.
+  - fold shifted_rule_in.
+    intros; simpl.
+    apply /orP; right.
+    change (n+m).+1 with (n.+1 + m).
+    auto.
+Qed.
+
+Lemma rule_in_mono n r l
+  : shifted_rule_in n r l -> forall r', shifted_rule_in n r%%!1 (r'::l).
+Proof.
+  intros.
+  apply: shifted_rule_in_cons.
+  change n.+1 with (1+n).
+  rewrite addnC.
+  by apply: unshift_rule_in_cons.
+Qed.
+
+Definition rule_in r (l : lang) : bool := shifted_rule_in 0 r l.
+Hint Unfold rule_in.
+
+Fixpoint shifted_is_nth n (r : rule) l m : bool :=
+  match m, l with
+  | _, [::] => false
+  | 0, r'::l' => (rule_constr_shift n r' == r)
+  | m'.+1, _::l' => shifted_is_nth n.+1 r l' m'
+  end.
+
+Lemma unshift_is_nth_cons n r l m
+  : shifted_is_nth n r l m -> forall n', shifted_is_nth (n + n') r%%!n' l m.
+Proof.
+  elim: m l n => //.
+  - case; simpl; auto.
+    intro_to is_true.
+    move /eqP <- => n'.
+    by rewrite rule_constr_shift_shift.
+  - intro_to seq.
+    case; simpl; auto.
+    intros.
+    change (n0 + n').+1 with (n0.+1 + n').
+    auto.
+Qed.
+
+Definition is_nth r l m := shifted_is_nth 0 r l m.
+Hint Unfold is_nth.
+  
 
 (* We could embed well-scopedness in bool, but well-typedness can be undecideable,
    so we leave it in Prop.
-   Some constructors take in more presuppositions than strictly necessary
-   (i.e. they can be derived from other arguments). This is a conscious design choice.
-   It is easier to devise secondary "constructor" functions that perform these
-   derivations than to do the mutually inductive proof that such derivations exist.
+   Expression constructors contain the index of the sort/term rule that proves them wf.
+   This is a deruijn version of how Jon Sterling does it
  *)
-Inductive wf_sort {p} : lang p -> ctx p -> exp p -> Prop :=
-| wf_sort_by : forall l c t,
-    wf_lang l ->
-    List.In ({| c|- t}) l ->
-    wf_sort l c t
-| wf_sort_subst : forall l c s c' t',
+Print List.
+Inductive wf_sort : lang -> ctx -> exp -> Prop :=
+| wf_sort_by : forall l c n s c',
+    is_nth ({| c' |- sort}) l n ->
     wf_subst l c s c' ->
-    wf_sort l c' t' ->
-    wf_sort l c t'[/s/]
-with le_sort {p} : lang p -> ctx p -> ctx p -> exp p -> exp p -> Prop :=
+    wf_sort l c (con n s)
+with le_sort : lang -> ctx -> ctx -> exp -> exp -> Prop :=
+(*TODO: constructor indices!!!
+ get right! should these get shifted?
+ answer: I think so, in every case where
+*)
 | le_sort_by : forall l c1 c2 t1 t2,
     wf_lang l ->
-    List.In ({< c1 <# c2 |- t1 <# t2}) l ->
+    rule_in ({< c1 <# c2 |- t1 <# t2}) l ->
     le_sort l c1 c2 t1 t2
 | le_sort_subst : forall l c1 c2 s1 s2 c1' c2' t1' t2',
     le_subst l c1 c2 s1 s2 c1' c2' ->
@@ -41,15 +431,11 @@ with le_sort {p} : lang p -> ctx p -> ctx p -> exp p -> exp p -> Prop :=
     le_sort l c1 c12 t1 t12 ->
     le_sort l c12 c2 t12 t2 ->
     le_sort l c1 c2 t1 t2
-with wf_term {p} : lang p -> ctx p -> exp p -> exp p -> Prop :=
-| wf_term_by : forall l c e t,
-    wf_lang l ->
-    List.In ({| c |- e .: t}) l ->
-    wf_term l c e t
-| wf_term_subst : forall l c s c' e' t',
+with wf_term : lang -> ctx -> exp -> exp -> Prop :=
+| wf_term_by : forall l c n s c' t,
+    is_nth ({| c' |- t}) l n ->
     wf_subst l c s c' ->
-    wf_term l c' e' t' ->
-    wf_term l c e'[/s/] t'[/s/]
+    wf_term l c (con n s) t[/s/]
 (* terms can be lifted to greater (less precise) types,
    but not the other way around
  *)
@@ -60,21 +446,20 @@ with wf_term {p} : lang p -> ctx p -> exp p -> exp p -> Prop :=
 | wf_term_var : forall l c t,
     wf_sort l c t ->
     wf_term l (t :: c) (var 0) t
-with le_term {p} : lang p ->
-                   ctx p -> ctx p ->
-                   exp p -> exp p ->
-                   exp p -> exp p -> Prop :=
+with le_term : lang ->
+               ctx -> ctx ->
+               exp -> exp ->
+               exp -> exp -> Prop :=
 | le_term_by : forall l c1 c2 e1 e2 t1 t2,
     wf_lang l ->
-    List.In ({< c1 <# c2|- e1 <# e2 .: t1 <# t2})%rule l ->
+    rule_in ({< c1 <# c2|- e1 <# e2 .: t1 <# t2}) l ->
     le_term l c1 c2 e1 e2 t1 t2
 | le_term_subst : forall l c1 c2 s1 s2 c1' c2' e1' e2' t1' t2',
     le_subst l c1 c2 s1 s2 c1' c2' ->
     le_term l c1' c2' e1' e2' t1' t2' ->
     le_term l c1 c2 e1'[/s1/] e2'[/s2/] t1'[/s1/] t2'[/s2/]
 | le_term_refl : forall l c e t,
-    wf_lang l ->
-    List.In ({| c |- e .: t })%rule l ->
+    wf_term l c e t ->
     le_term l c c e e t t
 | le_term_trans : forall l c1 c12 c2 e1 e12 e2 t1 t12 t2,
     le_term l c1 c12 e1 e12 t1 t12 ->
@@ -92,7 +477,7 @@ c1' < c2' |- e1 < e2 : t1' < t2'  \/
     le_sort l c1 c1' t1 t1' ->
     le_sort l c2 c2' t2 t2' ->
     le_term l c1' c2' e1 e2 t1' t2'
-with wf_subst {p} : lang p -> ctx p -> subst p ->  ctx p -> Prop :=
+with wf_subst : lang -> ctx -> subst -> ctx -> Prop :=
 | wf_subst_nil : forall l c,
     wf_ctx l c ->
     wf_subst l c [::] [::]
@@ -100,10 +485,10 @@ with wf_subst {p} : lang p -> ctx p -> subst p ->  ctx p -> Prop :=
     wf_subst l c s c' ->
     wf_term l c e t[/s/] ->
     wf_subst l c (e::s) (t::c')
-with le_subst {p} : lang p ->
-                    ctx p -> ctx p ->
-                    subst p -> subst p ->
-                    ctx p -> ctx p -> Prop :=
+with le_subst : lang ->
+                ctx -> ctx ->
+                subst -> subst ->
+                ctx -> ctx -> Prop :=
 | le_subst_nil : forall l c1 c2,
     le_ctx l c1 c2 ->
     le_subst l c1 c2 [::] [::] [::] [::]
@@ -111,26 +496,23 @@ with le_subst {p} : lang p ->
     le_subst l c1 c2 s1 s2 c1' c2' ->
     le_term l c1 c2 e1 e2 t1[/s1/] t2[/s2/] ->
     le_subst l c1 c2 (e1::s1) (e2::s2) (t1::c1') (t2 :: c2')
-with wf_ctx {p} : lang p -> ctx p -> Prop :=
+with wf_ctx : lang -> ctx -> Prop :=
 | wf_ctx_nil : forall l, wf_lang l -> wf_ctx l [::]
 | wf_ctx_cons : forall l c v,
     wf_sort l c v ->
     wf_ctx l (v::c)
-with le_ctx {p} : lang p -> ctx p -> ctx p -> Prop :=
+with le_ctx : lang -> ctx -> ctx -> Prop :=
 | le_ctx_nil : forall l, wf_lang l -> le_ctx l [::] [::]
 | le_ctx_cons : forall l c1 c2 v1 v2,
     le_sort l c1 c2 v1 v2 ->
     le_ctx l (v1::c1) (v2::c2)
-with wf_rule {p} : lang p -> rule p -> Prop :=
-| wf_sort_rule : forall l c t,
+with wf_rule : lang -> rule -> Prop :=
+| wf_sort_rule : forall l c,
     wf_ctx l c ->
-    (* TODO: require t (prefix) not in thy? interferes with monotonicity *)
-    wf_rule l ({| c |- t})
-| wf_term_rule : forall l c e t,
-    wf_ctx l c ->
+    wf_rule l ({| c |- sort})
+| wf_term_rule : forall l c t,
     wf_sort l c t ->
-    (* TODO: require e (prefix) not in thy? interferes with monotonicity *)
-    wf_rule l ({| c |- e .: t})
+    wf_rule l ({| c |- t})
 | le_sort_rule : forall l c1 c2 t1 t2,
     le_ctx l c1 c2 ->
     wf_sort l c1 t1 ->
@@ -141,7 +523,7 @@ with wf_rule {p} : lang p -> rule p -> Prop :=
     wf_term l c1 e1 t1 ->
     wf_term l c2 e2 t2 ->
     wf_rule l ({< c1 <# c2 |- e1 <# e2 .: t1 <# t2})
-with wf_lang {p} : lang p -> Prop :=
+with wf_lang : lang -> Prop :=
 | wf_lang_nil : wf_lang [::]
 | wf_lang_cons : forall l r, wf_rule l r -> wf_lang (r::l).
 Hint Constructors wf_sort.
@@ -160,21 +542,14 @@ Hint Constructors wf_lang.
    particularly for use when the proof must be inspected for well-foundedness
  *)
 
-Ltac get_polynomial :=
-  match goal with
-    p : polynomial |- _ => p
-  end.
-
 (* tac_map tactics push under "wf : (wf_X ...) |- ... -> (wf_X ...)" goals to the subterms 
    These tactics are meant to generate readable proof terms
 *)
 Ltac tac_map_wf_sort wf :=
   refine (match wf with
-           | wf_sort_by _ _ _ _ _ => _ (*TODO*)
-           | wf_sort_subst _ _ _ _ _ _ _ => _
+           | wf_sort_by _ _ _ _ _ _ _ => _ (*TODO*)
             end);
-  [ intros; eapply wf_sort_by
-  | intros; eapply wf_sort_subst].
+  intros; eapply wf_sort_by.
 
 
 Ltac tac_map_le_sort :=
