coq/langs/Subst.v
@@ -8,6 +8,152 @@ Set Bullet Behavior "Strict Subproofs".
 (* TODO: change from loads to imports *)
 From excomp Require Import Exp CoreDefs Core.
 
+Ltac easy_wf_lang :=
+  first [ constructor
+        |  econstructor; unfold is_nth; simpl; eauto];
+  let n := numgoals in
+  guard n < 2.
+
+Definition ctx_lang : lang :=
+  [:: {| [:: [2(*tp*)|]; [1(*ctx*)|]] |- (*C,t*) [1(*ctx*)|]};
+     {| [::] |- (*.*) [0 (*ctx*)|]};
+     {| [::] |- (*ctx*) sort };
+     {| [::] |- (*tp*) sort }].
+
+Lemma wf_ctx_lang : wf_lang ctx_lang.
+Proof.
+  pose p := eqP.
+  repeat easy_wf_lang.
+Qed.  
+
+Definition subst_lang : lang :=
+  [::
+    (* {| [:: [5(*tp*)|];[1(*var*)| var 1; var 0];[5(*tp*)|]; [4(*ctx*)|]]
+        |- (*S x*) [1(*var*)| [2(*C,t'*)| var 3; var 0];var 2]};
+     *){| [:: [4(*tp*)|]; [3(*ctx*)|]] |- (*Z*) [0(*var*)| [1(*C,t*)| var 1; var 0] ; var 0]};
+     {| [:: [3(*tp*)|]; [2(*ctx*)|]] |- (*var(C|-t)*) sort}]
+++ ctx_lang.
+(* TODO: substitutions, judgments, equalities *)
+
+Lemma wf_subst_lang : wf_lang subst_lang.
+Proof.
+  pose p := eqP.
+  pose cl := wf_ctx_lang.
+  repeat easy_wf_lang.
+  constructor.
+  constructor.
+  constructor.
+  repeat easy_wf_lang.
+  (*TODO: issue: seems to be a +1 that isn't happening in the var C,t substitution*)
+  give_up.
+  repeat easy_wf_lang.
+  
+
+  match goal with
+    |- wf_subst ?L _ _ _ =>
+    suff: wf_lang L
+  end.
+  give_up.
+  repeat constructor.
+  match goal with
+    |- wf_sort ?L _ _ =>
+    enough (wf_lang L)
+  end;[| repeat easy_wf_lang].
+  repeat easy_wf_lang.
+  constructor.
+  constructor.
+  repeat easy_wf_lang.
+  give_up.
+  unfold exp_subst; simpl.
+  change (0+3) with 3.
+  change [3|] with ([3|][/[:: var 1; var 0]/]).
+  eapply wf_term_by.
+  unfold is_nth; simpl. eauto.
+  simpl.
+  repeat easy_wf_lang.
+  econstructor; unfold is_nth; simpl; eauto.
+  
+
+
+
+  
+  give_up.
+  repeat easy_wf_lang.
+  repeat constructor.
+  econstructor; unfold is_nth; simpl; eauto.
+  repeat constructor.
+  econstructor; unfold is_nth; simpl; eauto.
+  
+  
+  
+  match goal with
+    |- wf_sort ?L _ _ =>
+    enough (wf_lang L)
+  end;repeat easy_wf_lang.
+  let n := numgoals in
+  idtac numgoals.
+  - move => wfl.
+    constructor.
+    give_up.
+    + constructor.
+      constructor.
+      constructor.
+  - do 2 easy_wf_lang.
+    + do 3 easy_wf_lang.
+      * repeat easy_wf_lang.
+      * repeat easy_wf_lang.
+        give_up.
+      * 
+        repeat constructor.
+        -- repeat easy_wf_lang.
+        -- unfold rule_in; simpl; eauto.
+ 
+    econstructor; unfold is_nth; simpl; eauto.
+      repeat constructor.
+      econstructor; unfold is_nth; simpl; eauto.
+      repeat constructor.
+      econstructor; unfold is_nth; simpl; eauto.
+      repeat constructor.
+      * econstructor; unfold is_nth; simpl; eauto.
+        repeat constructor.
+        econstructor; unfold is_nth; simpl; eauto.
+        repeat constructor.
+        econstructor; unfold is_nth; simpl; eauto.
+        repeat constructor.
+        econstructor; unfold is_nth; simpl; eauto.
+        repeat constructor.
+        econstructor; unfold is_nth; simpl; eauto.
+        repeat constructor.
+        econstructor; unfold is_nth; simpl; eauto.
+        repeat constructor.
+        econstructor; unfold is_nth; simpl; eauto.
+        repeat constructor;
+        econstructor; unfold is_nth; simpl; eauto;
+        repeat constructor.
+      *
+    
+
+Definition subst_lang : lang subst_syn :=
+  (* terms *)
+  [::
+     (* ctxts*)
+     {| [::] |- empty_ctxt' .: ctxt'};
+     {| [:: term_var ctxt' ; term_var tp' ] |- cons_ctxt' (var 0) (var 1) .: ctxt'} ;
+     (* variables *)
+     {| [:: term_var tp'] |- zv' .: var_srt'(judg' (@! ,, (var 0)) (var 0))};
+     {| [:: term_var (var_srt' (judg' (var 0) (var 1))); term_var ctxt'; term_var tp']
+        |- (sv' (var 0)) .: var_srt' (judg' (@! ,, (var 0)) (var 0))};
+     (* judgments *)
+     {| [:: term_var (var 0); term_var (var_srt' (var 0)); sort_var]
+        |- (var 0) .: (var 2)}
+  ] ++
+    (* sorts *)
+    [:: {| [:: term_var ctxt' ; term_var tp' ] |- judg' (var 0) (var 1)} ;
+       {| [:: sort_var ] |- var_srt' (var 0)};
+       {| [::] |- ctxt' };
+       {| [::] |- tp' }
+    ].
+
 Definition list_syn : polynomial :=
   [:: (unit, 0) (* nil *)
    ; (unit, 2) (* cons*)].
@@ -55,26 +201,8 @@ Definition var_srt' s :=  [{subst_syn} 9 | tt, [* s]].
 Notation "@!" := empty_ctxt'.
 Notation "C ,, t" := (cons_ctxt' C t) (at level 90).
 
-Definition subst_lang : lang subst_syn :=
-  (* terms *)
-  [::
-     (* ctxts*)
-     {| [::] |- empty_ctxt' .: ctxt'};
-     {| [:: term_var ctxt' ; term_var tp' ] |- cons_ctxt' (var 0) (var 1) .: ctxt'} ;
-     (* variables *)
-     {| [:: term_var tp'] |- zv' .: var_srt'(judg' (@! ,, (var 0)) (var 0))};
-     {| [:: term_var (var_srt' (judg' (var 0) (var 1))); term_var ctxt'; term_var tp']
-        |- (sv' (var 0)) .: var_srt' (judg' (@! ,, (var 0)) (var 0))};
-     (* judgments *)
-     {| [:: term_var (var 0); term_var (var_srt' (var 0)); sort_var]
-        |- (var 0) .: (var 2)}
-  ] ++
-    (* sorts *)
-    [:: {| [:: term_var ctxt' ; term_var tp' ] |- judg' (var 0) (var 1)} ;
-       {| [:: sort_var ] |- var_srt' (var 0)};
-       {| [::] |- ctxt' };
-       {| [::] |- tp' }
-    ].
+
+
 
 Lemma wf_subst_lang : wf_lang subst_lang.
 Proof.
@@ -83,9 +211,12 @@ Proof.
   constructor.
   constructor; constructor.
   - constructor; constructor.
+    change ctxt
+    eapply wf_sort_subst.
     constructor.
     Focus 2.
-    
+    simpl.
+    eauto.
 
   eauto.
   constructor.
